# Power rule
For finding a derivative of an equation

For example if the equation in f(x)=x^2:

Slip down the exponent of x in front of x = (2x^2)

Subtract one from the exponent of x = (2x^1)

Final result = 2x^1 == 2x

f(x) = 2x

Another example f(x)=3x^2

(3\*2)x^2 = 6x^2

6x^1 = 6x

f(x) = 6x

Final example f(x)=2x             ← remember if nothings there it will be ^1

(2\*1)x^1 = 2x^1

2x^0 = 2                             ← as it is to the power of 0 it will be = 1 which leads to another 2\*1

**Multiple Terms** 

(from now on y = 2x we will represent it as f’(x) = 2)

Power Rule formula for multiple terms : h’(x) = f’(x)g(x) + f(x)g’(x)

Chain rule : [https://youtu.be/YG15m2VwSjA](https://youtu.be/YG15m2VwSjA)
-------------------------------------------------------------------------